index: hide
name: The Multiplication Rule

If  *A* and  *B* are two events defined on a  **sample space**, then:  *P*( *A* AND  *B*) =  *P*( *B*) *P*( *A*| *B*).

This rule may also be written as:  *P*( *A*| *B*) = <math xmlns:bib="http://bibtexml.sf.net/" xmlns:q="http://cnx.rice.edu/qml/1.0" xmlns:md="http://cnx.rice.edu/mdml" xmlns:m="http://www.w3.org/1998/Math/MathML" xmlns:cnxorg="http://cnx.rice.edu/system-info" xmlns="http://cnx.rice.edu/cnxml"><mrow><mfrac><mrow><mi>P</mi><mo stretchy="false">(</mo><mi>A</mi><mtext> AND </mtext><mi>B</mi><mo stretchy="false">)</mo></mrow><mrow><mi>P</mi><mo stretchy="false">(</mo><mi>B</mi><mo stretchy="false">)</mo></mrow></mfrac></mrow></math>

(The probability of  *A* given  *B* equals the probability of  *A* and  *B* divided by the probability of  *B*.)

If  *A* and  *B* are  **independent**, then  *P*( *A*| *B*) =  *P*( *A*). Then  *P*( *A* AND  *B*) =  *P*( *A*| *B*) *P*( *B*) becomes  *P*( *A* AND  *B*) =  *P*( *A*) *P*( *B*).
