index: hide
name: The Central Limit Theorem for Sums - Introduction

Suppose  *X* is a random variable with a distribution that may be  *known or unknown* (it can be any distribution) and suppose:

  1.  *μX* = the mean of  *Χ*
  2.  *σΧ* = the standard deviation of  *X*

If you draw random samples of size  *n*, then as  *n* increases, the random variable Σ *X* consisting of sums tends to be  **normally distributed** and Σ *Χ* ~  *N*(( *n*)( *μΧ*), (<math xmlns:bib="http://bibtexml.sf.net/" xmlns:q="http://cnx.rice.edu/qml/1.0" xmlns:md="http://cnx.rice.edu/mdml" xmlns:m="http://www.w3.org/1998/Math/MathML" xmlns:cnxorg="http://cnx.rice.edu/system-info" xmlns="http://cnx.rice.edu/cnxml"> <mrow>  <msqrt>   <mi>n</mi>  </msqrt> </mrow></math>)( *σΧ*)).

 *The* **central limit theorem for sums** says that if you keep drawing larger and larger samples and taking their sums, the sums form their own normal distribution (the sampling distribution), which approaches a normal distribution as the sample size increases.  *The normal distribution has a mean equal to the original mean multiplied by the sample size and a standard deviation equal to the original standard deviation multiplied by the square root of the sample size.*

The random variable Σ *X* has the following  *z*-score associated with it:

  1. Σ *x* is one sum.
  2. <math xmlns:bib="http://bibtexml.sf.net/" xmlns:q="http://cnx.rice.edu/qml/1.0" xmlns:md="http://cnx.rice.edu/mdml" xmlns:m="http://www.w3.org/1998/Math/MathML" xmlns:cnxorg="http://cnx.rice.edu/system-info" xmlns="http://cnx.rice.edu/cnxml"> <mrow>  <mi>z</mi><mtext> = </mtext><mfrac>   <mrow>    <mi>Σ</mi><mi>x</mi><mo>–</mo><mo stretchy="false">(</mo><mi>n</mi><mo stretchy="false">)</mo><mo stretchy="false">(</mo><msub>     <mi>μ</mi>     <mi>X</mi>    </msub>    <mo stretchy="false">)</mo>   </mrow>   <mrow>    <mo stretchy="false">(</mo><msqrt>     <mi>n</mi>    </msqrt>    <mo stretchy="false">)</mo><mo stretchy="false">(</mo><msub>     <mi>σ</mi>     <mi>X</mi>    </msub>    <mo stretchy="false">)</mo>   </mrow>  </mfrac> </mrow></math>  (n)(μX) = the mean of ΣX 	      (    n      )(    σ    X      )    = standard deviation of      ΣX     	
