index: hide
name: Hess’s Law

There are two ways to determine the amount of heat involved in a chemical change: measure it experimentally, or calculate it from other experimentally determined enthalpy changes. Some reactions are difficult, if not impossible, to investigate and make accurate measurements for experimentally. And even when a reaction is not hard to perform or measure, it is convenient to be able to determine the heat involved in a reaction without having to perform an experiment.

This type of calculation usually involves the use of  **Hess’s law**, which states:  *If a process can be written as the sum of several stepwise processes, the enthalpy change of the total process equals the sum of the enthalpy changes of the various steps*. Hess’s law is valid because enthalpy is a state function: Enthalpy changes depend only on where a chemical process starts and ends, but not on the path it takes from start to finish. For example, we can think of the reaction of carbon with oxygen to form carbon dioxide as occurring either directly or by a two-step process. The direct process is written:

<math xmlns:q="http://cnx.rice.edu/qml/1.0" xmlns:m="http://www.w3.org/1998/Math/MathML" xmlns:bib="http://bibtexml.sf.net/" xmlns:md="http://cnx.rice.edu/mdml" xmlns="http://cnx.rice.edu/cnxml"><mrow><mtext>C</mtext><mo stretchy="false">(</mo><mi>s</mi><mo stretchy="false">)</mo><mo>+</mo><msub><mtext>O</mtext><mn>2</mn></msub><mo stretchy="false">(</mo><mi>g</mi><mo stretchy="false">)</mo><mspace width="0.2em"/><mo stretchy="false">⟶</mo><mspace width="0.2em"/><msub><mrow><mtext>CO</mtext></mrow><mn>2</mn></msub><mo stretchy="false">(</mo><mi>g</mi><mo stretchy="false">)</mo><mspace width="3em"/><mtext>Δ</mtext><msubsup><mi>H</mi><mrow><mn>298</mn></mrow><mo>°</mo></msubsup><mo>=</mo><mn>−394</mn><mspace width="0.2em"/><mtext>kJ</mtext></mrow></math>

In the two-step process, first carbon monoxide is formed:

<math xmlns:q="http://cnx.rice.edu/qml/1.0" xmlns:m="http://www.w3.org/1998/Math/MathML" xmlns:bib="http://bibtexml.sf.net/" xmlns:md="http://cnx.rice.edu/mdml" xmlns="http://cnx.rice.edu/cnxml"><mrow><mtext>C</mtext><mo stretchy="false">(</mo><mi>s</mi><mo stretchy="false">)</mo><mo>+</mo><mspace width="0.1em"/><mfrac><mn>1</mn><mn>2</mn></mfrac><msub><mtext>O</mtext><mn>2</mn></msub><mo stretchy="false">(</mo><mi>g</mi><mo stretchy="false">)</mo><mspace width="0.2em"/><mo stretchy="false">⟶</mo><mspace width="0.2em"/><mtext>CO</mtext><mo stretchy="false">(</mo><mi>g</mi><mo stretchy="false">)</mo><mspace width="3em"/><mtext>Δ</mtext><msubsup><mi>H</mi><mrow><mn>298</mn></mrow><mo>°</mo></msubsup><mo>=</mo><mn>−111</mn><mspace width="0.2em"/><mtext>kJ</mtext></mrow></math>

Then, carbon monoxide reacts further to form carbon dioxide:

<math xmlns:data="http://www.w3.org/TR/html5/dom.html#custom-data-attribute" xmlns:q="http://cnx.rice.edu/qml/1.0" xmlns:m="http://www.w3.org/1998/Math/MathML" xmlns:bib="http://bibtexml.sf.net/" xmlns:md="http://cnx.rice.edu/mdml" xmlns="http://cnx.rice.edu/cnxml"><mrow><mtext>CO</mtext><mo stretchy="false">(</mo><mi>g</mi><mo stretchy="false">)</mo><mo>+</mo><mspace width="0.1em"/><mfrac><mn>1</mn><mn>2</mn></mfrac><msub><mtext>O</mtext><mn>2</mn></msub><mo stretchy="false">(</mo><mi>g</mi><mo stretchy="false">)</mo><mspace width="0.2em"/><mo stretchy="false">⟶</mo><mspace width="0.2em"/><msub><mtext>CO</mtext><mn>2</mn></msub><mo stretchy="false">(</mo><mi>g</mi><mo stretchy="false">)</mo><mspace width="3em"/><mtext>Δ</mtext><msubsup><mi>H</mi><mrow><mn>298</mn></mrow><mo>°</mo></msubsup><mo>=</mo><mn>−283</mn><mspace width="0.2em"/><mtext>kJ</mtext></mrow></math>

The equation describing the overall reaction is the sum of these two chemical changes:

<math xmlns:q="http://cnx.rice.edu/qml/1.0" xmlns:m="http://www.w3.org/1998/Math/MathML" xmlns:bib="http://bibtexml.sf.net/" xmlns:md="http://cnx.rice.edu/mdml" xmlns="http://cnx.rice.edu/cnxml"><mtable columnalign="left"><mtr/><mtr><mtd><mtext>Step 1: C</mtext><mo stretchy="false">(</mo><mi>s</mi><mo stretchy="false">)</mo><mo>+</mo><mspace width="0.1em"/><mfrac><mn>1</mn><mn>2</mn></mfrac><msub><mtext>O</mtext><mn>2</mn></msub><mo stretchy="false">(</mo><mi>g</mi><mo stretchy="false">)</mo><mspace width="0.2em"/><mo stretchy="false">⟶</mo><mspace width="0.2em"/><mtext>CO</mtext><mo stretchy="false">(</mo><mi>g</mi><mo stretchy="false">)</mo></mtd></mtr><mtr><mtd><munder accentunder="true"><mrow><mtext>Step 2: CO</mtext><mo stretchy="false">(</mo><mi>g</mi><mo stretchy="false">)</mo><mo>+</mo><mspace width="0.1em"/><mfrac><mn>1</mn><mn>2</mn></mfrac><msub><mtext>O</mtext><mn>2</mn></msub><mo stretchy="false">(</mo><mi>g</mi><mo stretchy="false">)</mo><mspace width="0.2em"/><mo stretchy="false">⟶</mo><mspace width="0.2em"/><msub><mrow><mtext>CO</mtext></mrow><mn>2</mn></msub><mo stretchy="false">(</mo><mi>g</mi><mo stretchy="false">)</mo></mrow><mo stretchy="true">¯</mo></munder></mtd></mtr><mtr><mtd><mtext>Sum: C</mtext><mo stretchy="false">(</mo><mi>s</mi><mo stretchy="false">)</mo><mo>+</mo><mspace width="0.1em"/><mfrac><mn>1</mn><mn>2</mn></mfrac><msub><mtext>O</mtext><mn>2</mn></msub><mo stretchy="false">(</mo><mi>g</mi><mo stretchy="false">)</mo><mo>+</mo><mtext>CO</mtext><mo stretchy="false">(</mo><mi>g</mi><mo stretchy="false">)</mo><mo>+</mo><mspace width="0.1em"/><mfrac><mn>1</mn><mn>2</mn></mfrac><msub><mtext>O</mtext><mn>2</mn></msub><mo stretchy="false">(</mo><mi>g</mi><mo stretchy="false">)</mo><mspace width="0.2em"/><mo stretchy="false">⟶</mo><mspace width="0.2em"/><mtext>CO</mtext><mo stretchy="false">(</mo><mi>g</mi><mo stretchy="false">)</mo><mo>+</mo><msub><mtext>CO</mtext><mn>2</mn></msub><mo stretchy="false">(</mo><mi>g</mi><mo stretchy="false">)</mo></mtd></mtr></mtable></math>

Because the CO produced in Step 1 is consumed in Step 2, the net change is:

<math xmlns:q="http://cnx.rice.edu/qml/1.0" xmlns:m="http://www.w3.org/1998/Math/MathML" xmlns:bib="http://bibtexml.sf.net/" xmlns:md="http://cnx.rice.edu/mdml" xmlns="http://cnx.rice.edu/cnxml"><mrow><mtext>C</mtext><mo stretchy="false">(</mo><mi>s</mi><mo stretchy="false">)</mo><mo>+</mo><msub><mtext>O</mtext><mn>2</mn></msub><mo stretchy="false">(</mo><mi>g</mi><mo stretchy="false">)</mo><mspace width="0.2em"/><mo stretchy="false">⟶</mo><mspace width="0.2em"/><msub><mrow><mtext>CO</mtext></mrow><mn>2</mn></msub><mo stretchy="false">(</mo><mi>g</mi><mo stretchy="false">)</mo></mrow></math>

According to Hess’s law, the enthalpy change of the reaction will equal the sum of the enthalpy changes of the steps. We can apply the data from the experimental enthalpies of combustion in  to find the enthalpy change of the entire reaction from its two steps:

<math xmlns:q="http://cnx.rice.edu/qml/1.0" xmlns:m="http://www.w3.org/1998/Math/MathML" xmlns:bib="http://bibtexml.sf.net/" xmlns:md="http://cnx.rice.edu/mdml" xmlns="http://cnx.rice.edu/cnxml"><mtable columnalign="left"><mtr columnalign="left"><mtd columnalign="left"><mrow><mtext>C</mtext><mo stretchy="false">(</mo><mi>s</mi><mo stretchy="false">)</mo><mo>+</mo><mspace width="0.1em"/><mfrac><mn>1</mn><mn>2</mn></mfrac><msub><mtext>O</mtext><mn>2</mn></msub><mo stretchy="false">(</mo><mi>g</mi><mo stretchy="false">)</mo><mspace width="0.2em"/><mo stretchy="false">⟶</mo><mspace width="0.2em"/><mtext>CO</mtext><mo stretchy="false">(</mo><mi>g</mi><mo stretchy="false">)</mo></mrow></mtd><mtd columnalign="left"><mrow><mtext>Δ</mtext><msubsup><mi>H</mi><mrow><mn>298</mn></mrow><mo>°</mo></msubsup><mo>=</mo><mn>−111</mn><mspace width="0.2em"/><mtext>kJ</mtext></mrow></mtd></mtr><mtr columnalign="left"><mtd columnalign="left"><mrow><mfrac><mrow><mtext>CO</mtext><mo stretchy="false">(</mo><mi>g</mi><mo stretchy="false">)</mo><mo>+</mo><mspace width="0.1em"/><mfrac><mn>1</mn><mn>2</mn></mfrac><msub><mtext>O</mtext><mn>2</mn></msub><mo stretchy="false">(</mo><mi>g</mi><mo stretchy="false">)</mo><mspace width="0.2em"/><mo stretchy="false">⟶</mo><mspace width="0.2em"/><msub><mrow><mtext>CO</mtext></mrow><mn>2</mn></msub><mo stretchy="false">(</mo><mi>g</mi><mo stretchy="false">)</mo></mrow><mrow><mtext>C</mtext><mo stretchy="false">(</mo><mi>s</mi><mo stretchy="false">)</mo><mo>+</mo><msub><mtext>O</mtext><mn>2</mn></msub><mo stretchy="false">(</mo><mi>g</mi><mo stretchy="false">)</mo><mspace width="0.2em"/><mo stretchy="false">⟶</mo><mspace width="0.2em"/><msub><mrow><mtext>CO</mtext></mrow><mn>2</mn></msub><mo stretchy="false">(</mo><mi>g</mi><mo stretchy="false">)</mo><mspace width="1em"/></mrow></mfrac></mrow></mtd><mtd columnalign="left"><mrow><mfrac><mrow><mtext>Δ</mtext><msubsup><mi>H</mi><mrow><mn>298</mn></mrow><mo>°</mo></msubsup><mo>=</mo><mn>−283</mn><mspace width="0.2em"/><mtext>kJ</mtext></mrow><mrow><mtext>Δ</mtext><msubsup><mi>H</mi><mrow><mn>298</mn></mrow><mo>°</mo></msubsup><mo>=</mo><mn>−394</mn><mspace width="0.2em"/><mtext>kJ</mtext></mrow></mfrac></mrow></mtd></mtr></mtable></math>

The result is shown in {'Figure_5_3_HessCO2 Figure 5.3.HessCO2}. We see that Δ *H* of the overall reaction is the same whether it occurs in one step or two. This finding (overall Δ *H* for the reaction = sum of Δ *H* values for reaction “steps” in the overall reaction) is true in general for chemical and physical processes.


{image:'Figure_5_3_HessCO2}
        

Before we further practice using Hess’s law, let us recall two important features of Δ *H*.

  1. ΔH is directly proportional to the quantities of reactants or products. For example, the enthalpy change for the reaction forming 1 mole of NO2(g) is +33.2 kJ: <math xmlns:q="http://cnx.rice.edu/qml/1.0" xmlns:m="http://www.w3.org/1998/Math/MathML" xmlns:bib="http://bibtexml.sf.net/" xmlns:md="http://cnx.rice.edu/mdml" xmlns="http://cnx.rice.edu/cnxml"><mrow><mfrac><mn>1</mn><mn>2</mn></mfrac><msub><mtext>N</mtext><mn>2</mn></msub><mo stretchy="false">(</mo><mi>g</mi><mo stretchy="false">)</mo><mo>+</mo><msub><mtext>O</mtext><mn>2</mn></msub><mo stretchy="false">(</mo><mi>g</mi><mo stretchy="false">)</mo><mspace width="0.2em"/><mo stretchy="false">⟶</mo><mspace width="0.2em"/><msub><mrow><mtext>NO</mtext></mrow><mn>2</mn></msub><mo stretchy="false">(</mo><mi>g</mi><mo stretchy="false">)</mo><mspace width="3em"/><mtext>Δ</mtext><mstyle mathvariant="italic"><mtext>H</mtext></mstyle><mo>=</mo><mtext>+33.2 kJ</mtext></mrow></math> When 2 moles of NO2 (twice as much) are formed, the ΔH will be twice as large: <math xmlns:q="http://cnx.rice.edu/qml/1.0" xmlns:m="http://www.w3.org/1998/Math/MathML" xmlns:bib="http://bibtexml.sf.net/" xmlns:md="http://cnx.rice.edu/mdml" xmlns="http://cnx.rice.edu/cnxml"><mrow><msub><mtext>N</mtext><mn>2</mn></msub><mo stretchy="false">(</mo><mi>g</mi><mo stretchy="false">)</mo><mo>+</mo><mn>2</mn><msub><mtext>O</mtext><mn>2</mn></msub><mo stretchy="false">(</mo><mi>g</mi><mo stretchy="false">)</mo><mspace width="0.2em"/><mo stretchy="false">⟶</mo><mspace width="0.2em"/><mn>2</mn><msub><mrow><mtext>NO</mtext></mrow><mn>2</mn></msub><mo stretchy="false">(</mo><mi>g</mi><mo stretchy="false">)</mo><mspace width="3em"/><mtext>Δ</mtext><mstyle mathvariant="italic"><mtext>H</mtext></mstyle><mo>=</mo><mtext>+66.4 kJ</mtext></mrow></math> In general, if we multiply or divide an equation by a number, then the enthalpy change should also be multiplied or divided by the same number.
  2. ΔH for a reaction in one direction is equal in magnitude and opposite in sign to ΔH for the reaction in the reverse direction. For example, given that: <math xmlns:q="http://cnx.rice.edu/qml/1.0" xmlns:m="http://www.w3.org/1998/Math/MathML" xmlns:bib="http://bibtexml.sf.net/" xmlns:md="http://cnx.rice.edu/mdml" xmlns="http://cnx.rice.edu/cnxml"><mrow><msub><mtext>H</mtext><mn>2</mn></msub><mo stretchy="false">(</mo><mi>g</mi><mo stretchy="false">)</mo><mo>+</mo><msub><mrow><mtext>Cl</mtext></mrow><mn>2</mn></msub><mo stretchy="false">(</mo><mi>g</mi><mo stretchy="false">)</mo><mspace width="0.2em"/><mo stretchy="false">⟶</mo><mspace width="0.2em"/><mn>2</mn><mtext>HCl</mtext><mo stretchy="false">(</mo><mi>g</mi><mo stretchy="false">)</mo><mspace width="3em"/><mtext>Δ</mtext><mstyle mathvariant="italic"><mtext>H</mtext></mstyle><mo>=</mo><mn>−184.6</mn><mspace width="0.2em"/><mtext>kJ</mtext></mrow></math> Then, for the “reverse” reaction, the enthalpy change is also “reversed”: <math xmlns:q="http://cnx.rice.edu/qml/1.0" xmlns:m="http://www.w3.org/1998/Math/MathML" xmlns:bib="http://bibtexml.sf.net/" xmlns:md="http://cnx.rice.edu/mdml" xmlns="http://cnx.rice.edu/cnxml"><mrow><mn>2</mn><mtext>HCl</mtext><mo stretchy="false">(</mo><mi>g</mi><mo stretchy="false">)</mo><mspace width="0.2em"/><mo stretchy="false">⟶</mo><mspace width="0.2em"/><msub><mtext>H</mtext><mn>2</mn></msub><mo stretchy="false">(</mo><mi>g</mi><mo stretchy="false">)</mo><mo>+</mo><msub><mrow><mtext>Cl</mtext></mrow><mn>2</mn></msub><mo stretchy="false">(</mo><mi>g</mi><mo stretchy="false">)</mo><mspace width="3em"/><mtext>Δ</mtext><mstyle mathvariant="italic"><mtext>H</mtext></mstyle><mo>=</mo><mtext>+184.6 kJ</mtext></mrow></math>

Here is a less straightforward example that illustrates the thought process involved in solving many Hess’s law problems. It shows how we can find many standard enthalpies of formation (and other values of Δ *H*) if they are difficult to determine experimentally.

We also can use  **Hess’s law** to determine the enthalpy change of any reaction if the corresponding enthalpies of formation of the reactants and products are available. The stepwise reactions we consider are: (i) decompositions of the reactants into their component elements (for which the enthalpy changes are proportional to the negative of the enthalpies of formation of the reactants), followed by (ii) re-combinations of the elements to give the products (with the enthalpy changes proportional to the enthalpies of formation of the products). The standard enthalpy change of the overall reaction is therefore equal to: (ii) the sum of the standard enthalpies of formation of all the products plus (i) the sum of the negatives of the standard enthalpies of formation of the reactants. This is usually rearranged slightly to be written as follows, with ∑ representing “the sum of” and  *n* standing for the stoichiometric coefficients:

<math xmlns:q="http://cnx.rice.edu/qml/1.0" xmlns:m="http://www.w3.org/1998/Math/MathML" xmlns:bib="http://bibtexml.sf.net/" xmlns:md="http://cnx.rice.edu/mdml" xmlns="http://cnx.rice.edu/cnxml"><mrow><mtext>Δ</mtext><msubsup><mi>H</mi><mrow><mtext>reaction</mtext></mrow><mo>°</mo></msubsup><mo>=</mo><mstyle displaystyle="true"><mo>∑</mo><mi>n</mi></mstyle><mspace width="0.2em"/><mo>×</mo><mspace width="0.2em"/><mtext>Δ</mtext><msubsup><mi>H</mi><mtext>f</mtext><mo>°</mo></msubsup><mo stretchy="false">(</mo><mtext>products</mtext><mo stretchy="false">)</mo><mo>−</mo><mstyle displaystyle="true"><mo>∑</mo> <mi>n</mi></mstyle><mspace width="0.2em"/><mo>×</mo><mspace width="0.2em"/><mtext>Δ</mtext><msubsup><mi>H</mi><mtext>f</mtext><mo>°</mo></msubsup><mo stretchy="false">(</mo><mtext>reactants</mtext><mo stretchy="false">)</mo></mrow></math>

The following example shows in detail why this equation is valid, and how to use it to calculate the enthalpy change for a reaction of interest.
